lib/coq/Prompt.v
@@ -106,54 +106,46 @@ match l with
   foreachE xs vars body
 end.
 
-Fixpoint foreach_ZM_up' {rv e Vars} (from to step off : Z) (n : nat) `{ArithFact (0 <? step)} `{ArithFact (0 <=? off)} (vars : Vars) (body : forall (z : Z) `(ArithFact (from <=? z <=? to)), Vars -> monad rv Vars e) {struct n} : monad rv Vars e.
-exact (
+Fixpoint foreach_ZM_up' {rv e Vars} (from to step off : Z) (n : nat) (* 0 <? step *) (* 0 <=? off *) (vars : Vars) (body : forall (z : Z) (* from <=? z <=? to *), Vars -> monad rv Vars e) {struct n} : monad rv Vars e :=
   if sumbool_of_bool (from + off <=? to) then
     match n with
     | O => returnm vars
-    | S n => body (from + off) _ vars >>= fun vars => foreach_ZM_up' rv e Vars from to step (off + step) n _ _ vars body
+    | S n => body (from + off) vars >>= fun vars => foreach_ZM_up' from to step (off + step) n vars body
     end
-  else returnm vars).
-Defined.
+  else returnm vars.
 
-Fixpoint foreach_ZE_up' {e Vars} (from to step off : Z) (n : nat) `{ArithFact (0 <? step)} `{ArithFact (0 <=? off)} (vars : Vars) (body : forall (z : Z) `(ArithFact (from <=? z <=? to)), Vars -> e + Vars) {struct n} : e + Vars.
-exact (
+Fixpoint foreach_ZE_up' {e Vars} (from to step off : Z) (n : nat) (* 0 <? step *) (* 0 <=? off *) (vars : Vars) (body : forall (z : Z) (* from <=? z <=? to *), Vars -> e + Vars) {struct n} : e + Vars :=
   if sumbool_of_bool (from + off <=? to) then
     match n with
     | O => inr vars
-    | S n => body (from + off) _ vars >>$= fun vars => foreach_ZE_up' e Vars from to step (off + step) n _ _ vars body
+    | S n => body (from + off) vars >>$= fun vars => foreach_ZE_up' from to step (off + step) n vars body
     end
-  else inr vars).
-Defined.
+  else inr vars.
 
-Fixpoint foreach_ZM_down' {rv e Vars} (from to step off : Z) (n : nat) `{ArithFact (0 <? step)} `{ArithFact (off <=? 0)} (vars : Vars) (body : forall (z : Z) `(ArithFact (to <=? z <=? from)), Vars -> monad rv Vars e) {struct n} : monad rv Vars e.
-exact (
+Fixpoint foreach_ZM_down' {rv e Vars} (from to step off : Z) (n : nat) (* 0 <? step *) (* off <=? 0 *) (vars : Vars) (body : forall (z : Z) (* to <=? z <=? from *), Vars -> monad rv Vars e) {struct n} : monad rv Vars e :=
   if sumbool_of_bool (to <=? from + off) then
     match n with
     | O => returnm vars
-    | S n => body (from + off) _ vars >>= fun vars => foreach_ZM_down' _ _ _ from to step (off - step) n _ _ vars body
+    | S n => body (from + off) vars >>= fun vars => foreach_ZM_down' from to step (off - step) n vars body
     end
-  else returnm vars).
-Defined.
+  else returnm vars.
 
-Fixpoint foreach_ZE_down' {e Vars} (from to step off : Z) (n : nat) `{ArithFact (0 <? step)} `{ArithFact (off <=? 0)} (vars : Vars) (body : forall (z : Z) `(ArithFact (to <=? z <=? from)), Vars -> e + Vars) {struct n} : e + Vars.
-exact (
+Fixpoint foreach_ZE_down' {e Vars} (from to step off : Z) (n : nat) (* 0 <? step *) (* off <=? 0 *) (vars : Vars) (body : forall (z : Z) (* to <=? z <=? from *), Vars -> e + Vars) {struct n} : e + Vars :=
   if sumbool_of_bool (to <=? from + off) then
     match n with
     | O => inr vars
-    | S n => body (from + off) _ vars >>$= fun vars => foreach_ZE_down' _ _ from to step (off - step) n _ _ vars body
+    | S n => body (from + off) vars >>$= fun vars => foreach_ZE_down' from to step (off - step) n vars body
     end
-  else inr vars).
-Defined.
+  else inr vars.
 
-Definition foreach_ZM_up {rv e Vars} from to step vars body `{ArithFact (0 <? step)} :=
+Definition foreach_ZM_up {rv e Vars} from to step vars body (* 0 <? step *) :=
     foreach_ZM_up' (rv := rv) (e := e) (Vars := Vars) from to step 0 (S (Z.abs_nat (from - to))) vars body.
-Definition foreach_ZM_down {rv e Vars} from to step vars body `{ArithFact (0 <? step)} :=
+Definition foreach_ZM_down {rv e Vars} from to step vars body (* 0 <? step *) :=
     foreach_ZM_down' (rv := rv) (e := e) (Vars := Vars) from to step 0 (S (Z.abs_nat (from - to))) vars body.
 
-Definition foreach_ZE_up {e Vars} from to step vars body `{ArithFact (0 <? step)} :=
+Definition foreach_ZE_up {e Vars} from to step vars body (* 0 <? step *) :=
     foreach_ZE_up' (e := e) (Vars := Vars) from to step 0 (S (Z.abs_nat (from - to))) vars body.
-Definition foreach_ZE_down {e Vars} from to step vars body `{ArithFact (0 <? step)} :=
+Definition foreach_ZE_down {e Vars} from to step vars body (* 0 <? step *) :=
     foreach_ZE_down' (e := e) (Vars := Vars) from to step 0 (S (Z.abs_nat (from - to))) vars body.
 
 (*declare {isabelle} termination_argument foreachM = automatic*)
@@ -353,7 +345,7 @@ Definition choose_from_list {A} (descr : string) (xs : list A) : monad rv A E :=
   (* Use sufficiently many nondeterministically chosen bits and convert into an
      index into the list *)
   choose_range descr 0 (Z.of_nat (List.length xs) - 1) >>= fun idx =>
-  match List.nth_error xs (Z.to_nat (projT1 idx)) with
+  match List.nth_error xs (Z.to_nat idx) with
     | Some x => returnm x
     | None => Fail ("choose " ++ descr)
   end.
