lib/coq/String.v
@@ -76,16 +76,15 @@ Definition string_startswith s expected :=
   let prefix := String.substring 0 (String.length expected) s in
   generic_eq prefix expected.
 
-Definition string_drop s (n : Z) `{ArithFact (n >=? 0)} :=
+Definition string_drop s (n : Z) :=
   let n := Z.to_nat n in
   String.substring n (String.length s - n) s.
 
-Definition string_take s (n : Z) `{ArithFact (n >=? 0)} :=
+Definition string_take s (n : Z) :=
   let n := Z.to_nat n in
   String.substring 0 n s.
 
-Definition string_length s : {n : Z & ArithFact (n >=? 0)} :=
- build_ex (Z.of_nat (String.length s)).
+Definition string_length s : Z := Z.of_nat (String.length s).
 
 Definition string_append := String.append.
 
@@ -124,7 +123,7 @@ match s with
     else (acc, len)
   end
 end.
-Local Definition int_of (s : string) (base : Z) (len : nat) : option (Z * {n : Z & ArithFact (n >=? 0)}) :=
+Local Definition int_of (s : string) (base : Z) (len : nat) : option (Z * Z) :=
 match s with
 | EmptyString => None
 | String h t =>
@@ -134,7 +133,7 @@ match s with
     if i <? base
     then
     let (i, len') := more_digits t base i (S len) in
-    Some (i, build_ex (Z.of_nat len'))
+    Some (i, Z.of_nat len')
     else None
   end
 end.
@@ -142,7 +141,7 @@ end.
 (* I've stuck closely to OCaml's int_of_string, because that's what's currently
    used elsewhere. *)
 
-Definition maybe_int_of_prefix (s : string) : option (Z * {n : Z & ArithFact (n >=? 0)}) :=
+Definition maybe_int_of_prefix (s : string) : option (Z * Z) :=
 match s with
 | EmptyString => None
 | String "0" (String ("x"|"X") t) => int_of t 16 2
@@ -161,9 +160,7 @@ Definition maybe_int_of_string (s : string) : option Z :=
 match maybe_int_of_prefix s with
 | None => None
 | Some (i,len) =>
-  if projT1 len =? projT1 (string_length s)
-  then Some i
-  else None
+  if len =? string_length s then Some i else None
 end.
 
 Fixpoint n_leading_spaces (s:string) : nat :=
@@ -173,19 +170,18 @@ Fixpoint n_leading_spaces (s:string) : nat :=
   | _ => 0
   end.
 
-Definition n_leading_spaces_Z (s:string) : {n : Z & ArithFact (n >=? 0)} :=
-  build_ex (Z.of_nat (n_leading_spaces s)).
+Definition n_leading_spaces_Z (s:string) : Z := Z.of_nat (n_leading_spaces s).
 
-Definition opt_spc_matches_prefix s : option (unit * {n : Z & ArithFact (n >=? 0)}) :=
-  Some (tt, build_ex (Z.of_nat (n_leading_spaces s))).
+Definition opt_spc_matches_prefix s : option (unit * Z) :=
+  Some (tt, Z.of_nat (n_leading_spaces s)).
 
-Definition spc_matches_prefix s : option (unit * {n : Z & ArithFact (n >=? 0)}) :=
+Definition spc_matches_prefix s : option (unit * Z) :=
   match n_leading_spaces s with
   | O => None
-  | S n => Some (tt, build_ex (Z.of_nat (S n)))
+  | S n => Some (tt, Z.of_nat (S n))
   end.
 
-Definition hex_bits_n_matches_prefix sz `{ArithFact (sz >=? 0)} s : option (mword sz * {n : Z & ArithFact (n >=? 0)}) :=
+Definition hex_bits_n_matches_prefix sz s : option (mword sz * Z) :=
   match maybe_int_of_prefix s with
   | None => None
   | Some (n, len) =>
