lib/coq/Undefined.v
@@ -76,9 +76,9 @@ Definition undefined_unit (_:unit) : monad rv unit E := returnm tt.
 Definition undefined_bool (_:unit) : monad rv bool E := choose_bool "undefined_bool".
 Definition undefined_string (_:unit) : monad rv string E := choose_string "undefined_string".
 Definition undefined_int (_:unit) : monad rv Z E := choose_int "undefined_int".
-Definition undefined_nat (_:unit) : monad rv {n : Z & ArithFact (n >=? 0)} E := choose_nat "undefined_nat".
+Definition undefined_nat (_:unit) : monad rv Z E := choose_nat "undefined_nat".
 Definition undefined_real (_:unit) : monad rv _ E := choose_real "undefined_real".
-Definition undefined_range i j `{ArithFact (i <=? j)}: monad rv _ E := choose_range "undefined_range" i j.
+Definition undefined_range i j : monad rv Z E := choose_range "undefined_range" i j.
 Definition undefined_bitvector n : monad rv (mword n) E := choose_bitvector "undefined_bitvector" n.
 
 Definition undefined_vector {T} n `{Inhabited T} (a:T) : monad rv (vec T n) E := returnm (vec_init a n).
